Isabelle2/MultiPaxosL1Correctness.thy
@@ -1,43 +1,118 @@
+section {* MultiPaxosL1 refines AbstractMultiPaxos7 *}
+
 theory MultiPaxosL1Correctness
 imports MultiPaxosL1 AbstractMultiPaxos7 "../../IO-Automata/Simulations"
 begin
 
-locale l1_correctness = mp1
+locale l1_correctness = mp1 acceptors quorums learners for acceptors quorums learners +
+  fixes the_ioa :: "(('v,'a)mp_state, ('v,'a,'b)mp_action) ioa"
+  defines "the_ioa \<equiv> mp_ioa"
+    -- {* Here I just made this definition to "bind" all type variables so that I don't get
+      weird behavior in apply scripts. *}
 begin
 
 interpretation amp: amp_ioa acceptors quorums learners .
 
-fun rn where 
-  "rn (Propose v) = Some (amp.Propose v)"
-| "rn (Learn i v l) = Some (amp.Learn i v l)"
-| "rn (Vote a q i v) = Some (amp.Vote a q i v)"
-| "rn (JoinBallot a i) = Some (amp.JoinBallot a i)"
-| "rn (Suggest a v i b q) = None"
+context begin
+
+subsection {* Renaming the IOAs to a common signature *}
+
+private
+datatype ('vv,'aa,'ll)common_act =
+  Learn nat 'vv 'll
+| Propose 'vv
+| Vote 'aa nat 'vv
+| VoteQ 'aa "'aa set" nat 'vv
+| JoinBallot 'aa nat
+| Suggest 'aa 'vv nat nat "'aa set"
+
+fun rn_1 where   
+  "rn_1 (Propose v) = Some (mp_action.Propose v)"
+| "rn_1 (Learn i v l) = Some (mp_action.Learn i v l)"
+| "rn_1 (VoteQ a q i v) = None"
+| "rn_1 (JoinBallot a i) = Some (mp_action.JoinBallot a i)"
+| "rn_1 (Vote a i v) = Some (mp_action.Vote a i v)"
+| "rn_1 (Suggest a v i b q) = Some (mp_action.Suggest a v i b q)"
+
+fun rn_2 where 
+  "rn_2 (Propose v) = Some (amp.Propose v)"
+| "rn_2 (Learn i v l) = Some (amp.Learn i v l)"
+| "rn_2 (VoteQ a q i v) = Some (amp.Vote a q i v)"
+| "rn_2 (JoinBallot a i) = Some (amp.JoinBallot a i)"
+| "rn_2 (Vote a i v) = None"
+| "rn_2 (Suggest a v i b q) = None"
+
+definition amp_ioa_2 :: "(('v, 'a) amp_state, ('v, 'a, 'b) common_act) ioa" where
+  "amp_ioa_2 \<equiv> rename amp.amp_ioa rn_2"
+
+definition mp_ioa_2 :: "(('v, 'a) mp_state, ('v, 'a, 'b) common_act) ioa" where
+  "mp_ioa_2 \<equiv> rename mp_ioa rn_1"
+
+lemmas ioa_simps = rename_def rename_set_def refines_def is_trans_def trace_def
+  externals_def schedule_def filter_act_def
+lemmas simps = amp_ioa_2_def mp_ioa_2_def amp.simps simps ioa_simps
+declare simps[inv_proofs_defs]
+
+definition inv1 :: "('v, 'a) mp_state \<Rightarrow> bool" where 
+  "inv1 s \<equiv> \<forall> i b v . let sug = suggestion s i b in 
+    sug = Some v \<longrightarrow> (v \<in> mp_state.propCmd s 
+      \<and> (\<exists> q \<in> quorums . proved_safe_at s i q b v
+          \<and> (\<forall> a \<in> q . mp_state.ballot s a \<ge> Some b)))"
+
+definition inv3 :: "('v, 'a) mp_state \<Rightarrow> bool" where 
+  -- {* votes are always equal to the suggestion. Why do I need this? *}
+  "inv3 s \<equiv> \<forall> (a::'a) i b .
+    case mp_state.vote s i a b of Some v \<Rightarrow> 
+      (case suggestion s i b of Some w \<Rightarrow> v = w | None \<Rightarrow> False)
+    | None \<Rightarrow> True"
+
+lemmas inv_defs = inv3_def inv1_def
+
+declare option.splits[split]
+
+lemma inv3[invs]:"invariant mp_ioa inv3"
+  -- {* Why is this one so painful? *}
+apply (try_solve_inv2 inv_proofs_defs:inv_proofs_defs inv_defs ballot_array.conservative_array_def
+  ballot_array.conservative_def)
+apply (case_tac a; rm_reachable)
+apply ((auto simp add:inv_proofs_defs inv_defs ballot_array.conservative_array_def
+  ballot_array.conservative_def))
+apply (metis option.collapse)
+apply (metis option.collapse)
+apply (metis option.collapse)
+apply (metis option.collapse)
+apply (metis option.collapse)
+apply (metis option.collapse)
+apply (metis option.collapse)
+defer
+apply (metis option.collapse)
+apply (metis option.collapse)
+by (metis option.simps(3))
+
+lemma inv2[invs]:"invariant mp_ioa inv1"
+apply (try_solve_inv2 inv_proofs_defs:inv_proofs_defs inv_defs ballot_array.conservative_array_def
+  ballot_array.conservative_def)
+apply (case_tac a; (auto simp add:inv_proofs_defs inv_defs ballot_array.conservative_array_def
+  ballot_array.conservative_def; fail)?; rm_reachable)
+subgoal premises p for s t act a _ i v
+proof - 
+  have "do_vote a i v s t" oops
+
+subsection {* A refinement mapping proof *}
 
 definition f where "f s \<equiv> \<lparr>
     propCmd = mp_state.propCmd s,
     ballot = mp_state.ballot s,
     vote = mp_state.vote s \<rparr>"
 
-definition amp_ioa_2 where
-  "amp_ioa_2 \<equiv> rename amp.amp_ioa rn"
-
-lemmas ioa_simps = rename_def rename_set_def refines_def is_trans_def trace_def
-  externals_def schedule_def filter_act_def
-lemmas simps = amp_ioa_2_def amp.simps f_def simps ioa_simps
-
-definition inv1 where 
-  "inv1 s \<equiv> let v = suggestion s in 
-    (v \<in> propCmd s \<and> (\<exists> q \<in> quorums . True))"
-
-lemma "is_ref_map f mp_ioa amp_ioa_2"
+lemma "is_ref_map f mp_ioa_2 amp_ioa_2"
 proof (auto simp add:is_ref_map_def)
   fix s
-  assume "s \<in> start mp_ioa"
-  thus "f s \<in> start amp_ioa_2" by (simp add:ioa_simps simps)
+  assume "s \<in> start mp_ioa_2"
+  thus "f s \<in> start amp_ioa_2" by (simp add:ioa_simps simps f_def)
 next
   fix s t a 
-  assume "reachable mp_ioa s" and trans:"s \<midarrow>a\<midarrow>mp_ioa\<longrightarrow> t"
+  assume "reachable mp_ioa_2 s" and trans:"s \<midarrow>a\<midarrow>mp_ioa_2\<longrightarrow> t"
   show "\<exists>aa b. refines (aa, b) s a t amp_ioa_2 f"
   proof (cases a)
     case (Propose v)
@@ -45,7 +120,7 @@ next
     let ?a = "[(Propose v, f t)]"
     show ?thesis using Propose trans
         apply (intro exI[where ?x="?s"] exI[where ?x="?a"], auto simp add:refines_def)
-      apply (auto simp add:simps)
+      apply (auto simp add:simps f_def)
     done
   next
     case (Learn x y z)
@@ -53,7 +128,7 @@ next
     let ?a = "[(Learn x y z, f t)]"
     show ?thesis using Learn trans
         apply (intro exI[where ?x="?s"] exI[where ?x="?a"], auto simp add:refines_def)
-      apply (auto simp add:simps)
+      apply (auto simp add:simps  f_def)
     done
   next
   defer
@@ -62,7 +137,7 @@ next
     let ?a = "[(JoinBallot x y, f t)]"
     show ?thesis using JoinBallot trans
         apply (intro exI[where ?x="?s"] exI[where ?x="?a"], auto simp add:refines_def)
-      apply (auto simp add:simps)
+      apply (auto simp add:simps f_def)
     done
   next
     case (Suggest x1 x2 x3 x4 x5)
@@ -70,12 +145,12 @@ next
     let ?a = "[]"
     show ?thesis using Suggest trans
         apply (intro exI[where ?x="?s"] exI[where ?x="?a"], auto simp add:refines_def)
-      apply (auto simp add:simps)
+      apply (auto simp add:simps f_def)
     done
   next (* Now I need an invariant saying that the suggestion comes from a quorum with all the right properties. *) oops
   
 
-lemma "traces mp_ioa \<subseteq> traces amp_ioa_2" oops
+lemma "traces mp_ioa_2 \<subseteq> traces amp_ioa_2" oops
 
 end
 
